Remove axiomatization

operations/Corecursor.thy
@@ -7,6 +7,10 @@ begin
 lemma rel_set_reflI: "(\<And>a. a \<in> A \<Longrightarrow> r a a) \<Longrightarrow> rel_set r A A"
   by (auto simp: rel_set_def)
 
+definition asSS :: "('a \<Rightarrow> 'a) \<Rightarrow> 'a \<Rightarrow> 'a" where
+  "asSS f \<equiv> if |supp f| <o |UNIV::'a set| then f else id"
+
+
 (* Definitions *)
 
 locale COREC =
@@ -40,17 +44,6 @@ locale COREC =
     and valid_Umap: "bij f \<Longrightarrow> |supp (f::'a::var \<Rightarrow> 'a)| <o |UNIV::'a set| \<Longrightarrow> valid_U d \<Longrightarrow> valid_U (Umap f d)"
     and valid_Udtor: "\<And>x. valid_U d \<Longrightarrow> x \<in> Udtor d \<Longrightarrow> pred_term_pre (pred_sum (\<lambda>_. True) valid_U)  (pred_sum (\<lambda>_. True) valid_U) x"
 begin
-
-definition suitable' ::  "('u \<Rightarrow> ('a, 'a, 'a raw_term + 'u, 'a raw_term + 'u) term_pre set) \<Rightarrow> ('u \<Rightarrow> ('a, 'a, 'a raw_term + 'u,'a raw_term + 'u) term_pre) \<Rightarrow> bool" where
-  "suitable' Utor pick \<equiv> \<forall> d. pick d \<in> Utor d"
-definition f' :: "('u \<Rightarrow> ('a::var,'a,'a raw_term + 'u,'a raw_term + 'u) term_pre) \<Rightarrow> 'u => 'a raw_term" where
-  "f' pick \<equiv> corec_raw_term pick"
-definition pick0' :: "('u \<Rightarrow> ('a, 'a, 'a raw_term + 'u, 'a raw_term + 'u) term_pre set) \<Rightarrow> 'u \<Rightarrow> ('a, 'a, 'a raw_term + 'u, 'a raw_term + 'u) term_pre" where
-  "pick0' Utor \<equiv> SOME pick. suitable' Utor pick"
-definition f0' :: "'u \<Rightarrow> 'a raw_term" where
-  "f0' \<equiv> f' (pick0' (\<lambda>(d::'u). map_term_pre id id (map_sum TT_rep id) (map_sum TT_rep id) ` Udtor d))"
-definition COREC :: "'u \<Rightarrow> 'a term" where
-  "COREC d = TT_abs (f0' d)"
 
 lemma Umap_id: "valid_U d \<Longrightarrow> Umap id d = d"
   apply (rule Umap_cong0)
@@ -161,145 +154,25 @@ proof -
     done
 qed
 
-lemma COREC_DDTOR: "valid_U d \<Longrightarrow> X \<in> Udtor d \<Longrightarrow> COREC d = term_ctor (map_term_pre id id (case_sum id COREC) (case_sum id COREC) X)"
-  sorry
-
-  lemma COREC_mmapD: "valid_U d \<Longrightarrow> bij u \<Longrightarrow> |supp u| <o |UNIV::'a set| \<Longrightarrow> COREC (Umap u d) = permute_term u (COREC d)"
-    sorry
-  lemma  COREC_FFVarsD: "valid_U d \<Longrightarrow> FVars_term (COREC d) \<subseteq> UFVars d"
-    sorry
-end
-
-(* The domain type: *)
-typedecl 'a U
-
-consts Udtor :: "'a::var U \<Rightarrow> ('a, 'a, 'a term + 'a U, 'a term + 'a U) term_pre set"
-consts Umap :: "('a \<Rightarrow> 'a) \<Rightarrow> 'a::var U \<Rightarrow> 'a U"
-consts UFVars :: "'a::var U \<Rightarrow> 'a set"
-
-axiomatization where
-  (* The destructor is non-empty and deterministic modulo a renaming: *)
-  Udtor_ne: "\<And>d. Udtor d \<noteq> {}"
-  and
-  alpha_Udtor: "\<And>X X' d. {X,X'} \<subseteq> Udtor d \<Longrightarrow>
-\<exists>u. bij (u::'a::var \<Rightarrow> 'a) \<and> |supp u| <o |UNIV::'a set| \<and> id_on ((\<Union>z \<in> set3_term_pre X. case_sum FVars_term UFVars z) - set2_term_pre X) u \<and>
-     map_term_pre id u (map_sum (permute_term u) (Umap u)) id X = X'"
-  and
-  (* The dual of the first block of assumptions from Norrish's paper:   *)
-  UFVars_Udtor:
-  "\<And> d X. X \<in> Udtor d \<Longrightarrow>
-  set1_term_pre X \<union> (\<Union>z \<in> set4_term_pre X. case_sum FVars_term UFVars z) \<union>
-   ((\<Union>z \<in> set3_term_pre X. case_sum FVars_term UFVars z) - set2_term_pre X) \<subseteq>
-  UFVars d"
-  and
-  (* The dual of the third block: *)
-  Umap_Udtor: "\<And>u d.
-  bij (u::'a\<Rightarrow>'a) \<Longrightarrow> |supp u| <o |UNIV::'a::var set| \<Longrightarrow>
-  Udtor (Umap u d) \<subseteq>
-  image
-    (map_term_pre u u (map_sum (permute_term u) (Umap u)) (map_sum (permute_term u) (Umap u)))
-    (Udtor d)"
-  and Umap_comp0: "bij f \<Longrightarrow> |supp (f::'a::var \<Rightarrow> 'a)| <o |UNIV::'a set| \<Longrightarrow> bij g \<Longrightarrow> |supp (g::'a::var \<Rightarrow> 'a)| <o |UNIV::'a set|
-  \<Longrightarrow> Umap f \<circ> Umap g = Umap (f \<circ> g)"
-  and Umap_cong0: "bij f \<Longrightarrow> |supp (f::'a::var \<Rightarrow> 'a)| <o |UNIV::'a set|
-  \<Longrightarrow> (\<And>a. a \<in> UFVars d \<Longrightarrow> f a = a) \<Longrightarrow> Umap f d = d"
-  (*and Umap_UFVars: "bij f \<Longrightarrow> |supp (f::'a::var \<Rightarrow> 'a)| <o |UNIV::'a set|
-  \<Longrightarrow> UFVars (Umap f d) = f ` UFVars d"*)
-
-lemma Umap_id0: "Umap id = id"
-  apply (rule ext)
-  apply (rule trans[OF _ id_apply[symmetric]])
-  apply (rule Umap_cong0)
-    apply (rule bij_id supp_id_bound)+
-  apply (rule id_apply)
-  done
-
-(*
-D \<Rightarrow> U
-TT \<Rightarrow> term
-F \<Rightarrow> term_pre
-vvar_TT \<Rightarrow> var
-
-FFVars \<Rightarrow> FVars_term
-FFVarsD \<Rightarrow> UFVars
-DDTOR \<Rightarrow> Udtor
-mmapD \<Rightarrow> Umap
-
-set2_F \<Rightarrow> set2_term_pre
-if set has minus \<Rightarrow> set3_term_pre
-if not \<Rightarrow> set4_term_pre
-*)
-
-(* Defined analogously to the FVarsB: *)
-(* TODO(ozkutuk): rename this? FFVarsBD \<rightarrow> UFVarsB? *)
-definition FFVarsBD :: "('a::var, 'a, 'a term + 'a U, 'a term + 'a U) term_pre \<Rightarrow> 'a set" where
+definition FFVarsBD :: "('a::var, 'a, 'a term + 'u, 'a term + 'u) term_pre \<Rightarrow> 'a set" where
   "FFVarsBD X \<equiv> (\<Union>z \<in> set3_term_pre X. case_sum FVars_term UFVars z) - set2_term_pre X"
 
-thm alpha_Udtor
 lemmas Udtor_Umap = alpha_Udtor[folded FFVarsBD_def]
 lemmas FVars_term_Udtor = UFVars_Udtor[folded FFVarsBD_def]
-
-lemma Umap_id[simp,intro!]: "Umap id d = d"
-  apply (rule trans[OF Umap_id0[THEN fun_cong]])
-  apply (rule id_apply)
-  done
-
-lemma Umap_comp:
-  "bij (u::'a\<Rightarrow>'a) \<Longrightarrow> |supp u| <o |UNIV::('a::var) set| \<Longrightarrow> bij v \<Longrightarrow> |supp v| <o |UNIV::'a set| \<Longrightarrow>
- Umap (u o v) d = Umap u (Umap v d)"
-  apply (subst Umap_comp0[symmetric])
-      apply assumption+
-  apply (rule comp_apply)
-  done
-
-lemma Umap_Udtor_strong:
-  assumes u: "bij (u::'a::var\<Rightarrow>'a)" "|supp u| <o |UNIV::'a set|"
-  shows
-    "Udtor (Umap u d) =
- image
-   (map_term_pre u u (map_sum (permute_term u) (Umap u)) (map_sum (permute_term u) (Umap u)))
-   (Udtor d)"
-proof -
-  have x: "d = Umap (inv u) (Umap u d)"
-    apply (rule sym)
-    apply (rule trans[OF Umap_comp[symmetric]])
-        apply (rule bij_imp_bij_inv supp_inv_bound assms)+
-    apply (subst inv_o_simp1, rule assms)+
-    apply (rule trans[OF Umap_id0[THEN fun_cong]])
-    apply (rule id_apply)
-    done
-  show ?thesis
-    apply (rule subset_antisym)
-     apply (rule Umap_Udtor[OF assms])
-    apply (subst x)
-    apply (rule image_subsetI)
-    apply (drule Umap_Udtor[THEN subsetD, rotated -1])
-      apply (rule bij_imp_bij_inv supp_inv_bound assms)+
-    apply (erule imageE)
-    apply hypsubst
-    apply (rule iffD2[OF arg_cong2[OF _ refl, of _ _ "(\<in>)"]])
-     apply (rule term_pre.map_comp)
-          apply (rule bij_imp_bij_inv supp_inv_bound assms)+
-    apply (unfold map_sum.comp)
-    apply (subst inv_o_simp2 permute_comp0s Umap_comp0, (rule bij_imp_bij_inv supp_inv_bound assms)+)+
-    apply (unfold Umap_id0 permute_id0s map_sum.id term_pre.map_id)
-    apply assumption
-    done
-qed
 
 (*************************************)
 (* The raw-term-based model infrastructure *)
 
-definition Utor :: "'a::var U \<Rightarrow> ('a, 'a, 'a raw_term + 'a U, 'a raw_term + 'a U) term_pre set" where
+definition Utor :: "'u \<Rightarrow> ('a::var, 'a, 'a raw_term + 'u, 'a raw_term + 'u) term_pre set" where
   "Utor d \<equiv>  map_term_pre id id (map_sum TT_rep id) (map_sum TT_rep id) ` (Udtor d)"
 
-abbreviation raw_Umap :: "('a::var \<Rightarrow> 'a) \<Rightarrow> 'a U \<Rightarrow> 'a U" where
+abbreviation raw_Umap :: "('a::var \<Rightarrow> 'a) \<Rightarrow> 'u \<Rightarrow> 'u" where
   "raw_Umap \<equiv> Umap"
 
-abbreviation raw_UFVars :: "'a::var U \<Rightarrow> 'a set" where
+abbreviation raw_UFVars :: "'u \<Rightarrow> 'a::var set" where
   "raw_UFVars \<equiv> UFVars"
 
-definition raw_UFVarsBD :: "('a::var, 'a, 'a raw_term + 'a U, 'a raw_term + 'a U) term_pre \<Rightarrow> 'a set" where
+definition raw_UFVarsBD :: "('a::var, 'a, 'a raw_term + 'u, 'a raw_term + 'u) term_pre \<Rightarrow> 'a set" where
   "raw_UFVarsBD X \<equiv> \<Union>(case_sum FVars_raw_term raw_UFVars ` set3_term_pre X) - set2_term_pre X"
 
 lemmas raw_UFVars_def2 = trans[OF meta_eq_to_obj_eq[OF FVars_term_def[of "TT_abs _"]] alpha_FVars[OF TT_rep_abs], symmetric]
@@ -332,10 +205,8 @@ lemma abs_rep_id: "TT_abs o TT_rep = id"
   apply (rule refl)
   done
 
-definition asSS :: "('a \<Rightarrow> 'a) \<Rightarrow> 'a \<Rightarrow> 'a" where
-  "asSS f \<equiv> if |supp f| <o |UNIV::'a set| then f else id"
-
 lemma DTOR_mapD:
+  assumes "valid_U d"
   shows "{X,X'} \<subseteq> Utor d \<Longrightarrow> \<exists>u. bij (u::'a::var\<Rightarrow>'a) \<and> |supp u| <o |UNIV::'a set| \<and> id_on (raw_UFVarsBD X) u \<and>
      mr_rel_term_pre id u
        (rel_sum (\<lambda> t t'. alpha_term (permute_raw_term u t) t') (\<lambda> d d'. raw_Umap u d = d'))
@@ -345,7 +216,7 @@ lemma DTOR_mapD:
   apply (unfold image_insert image_empty Utor_def image_comp)
   apply (subst (asm) term_pre.map_comp0[symmetric], (rule supp_id_bound bij_id)+)
   apply (unfold id_o map_sum.comp abs_rep_id map_sum.id term_pre.map_id0 image_id)
-  apply (drule alpha_Udtor)
+  apply (drule alpha_Udtor[OF assms])
   apply (erule exE conjE)+
   apply (subst (asm) term_pre.set_map term_pre.map_comp, (rule supp_id_bound bij_id | assumption)+)+
   apply (unfold image_id id_o o_id map_sum.comp)
@@ -385,9 +256,9 @@ lemma DTOR_mapD:
   done
 
 lemma Utor_ne:
-  "Utor d \<noteq> {}"
+  "valid_U d \<Longrightarrow> Utor d \<noteq> {}"
   by (unfold Utor_def arg_cong[OF image_is_empty, of Not])
-    (rule Udtor_ne)
+    (erule Udtor_ne)
 
 lemma Utor_abs_Udtor: "X \<in> Utor d \<Longrightarrow> map_term_pre id id (map_sum TT_abs id) (map_sum TT_abs id) X \<in> Udtor d"
   apply (unfold Utor_def)
@@ -403,13 +274,6 @@ lemma Utor_abs_Udtor: "X \<in> Utor d \<Longrightarrow> map_term_pre id id (map_
   apply assumption
   done
 
-(*lemma raw_UFVars_def2_comp: "FVars_raw_term = FVars_term \<circ> TT_abs"
-  apply (unfold raw_UFVars_def2)
-  apply (unfold comp_apply)
-  apply (rule refl)
-  done
-*)
-
 lemma aux_raw_UFVars_Utor: "case_sum FVars_term raw_UFVars ` set4_term_pre (map_term_pre id id (map_sum TT_abs id) (map_sum TT_abs id) X) =
        case_sum FVars_raw_term raw_UFVars ` set4_term_pre X"
   apply (unfold raw_UFVars_def2)
@@ -421,8 +285,9 @@ lemma aux_raw_UFVars_Utor: "case_sum FVars_term raw_UFVars ` set4_term_pre (map_
   done
 
 lemma raw_UFVars_Utor:
-  "X \<in> Utor d \<Longrightarrow> set1_term_pre X \<union> \<Union>(case_sum FVars_raw_term raw_UFVars ` set4_term_pre X) \<union> raw_UFVarsBD X \<subseteq> raw_UFVars d"
-  apply (drule FVars_term_Udtor[OF Utor_abs_Udtor])
+  assumes "valid_U d"
+  shows "X \<in> Utor d \<Longrightarrow> set1_term_pre X \<union> \<Union>(case_sum FVars_raw_term raw_UFVars ` set4_term_pre X) \<union> raw_UFVarsBD X \<subseteq> raw_UFVars d"
+  apply (drule FVars_term_Udtor[OF assms Utor_abs_Udtor])
   apply (unfold FVarsBD_FFVarsBD)
   apply (subst (asm) term_pre.set_map, (rule supp_id_bound bij_id)+)
   apply (subst(asm) aux_raw_UFVars_Utor)
@@ -432,6 +297,7 @@ lemma raw_UFVars_Utor:
 
 lemma raw_Umap_Utor:
   assumes u: "bij (u::'a\<Rightarrow>'a)" "|supp u| <o |UNIV::'a::var set|"
+    and valid_d: "valid_U d"
   shows
     "rel_set
   (mr_rel_term_pre u u
@@ -441,6 +307,7 @@ lemma raw_Umap_Utor:
  (Utor (raw_Umap u d))"
   apply (unfold Utor_def)
   apply (subst Umap_Udtor_strong[OF u, of d])
+  apply (rule valid_d)
   apply (subst image_comp)
   apply (subst term_pre.map_comp0[symmetric])
       apply (rule assms supp_id_bound bij_id)+
@@ -471,16 +338,16 @@ lemma raw_Umap_Utor:
   apply (rule refl)
   done
 
-(*    *)
-
-
-definition suitable ::  "('a U \<Rightarrow> ('a::var, 'a, 'a raw_term + 'a U,'a raw_term + 'a U) term_pre) \<Rightarrow> bool" where
-  "suitable pick \<equiv> \<forall> d. pick d \<in> Utor d"
-
-definition f :: "('a U \<Rightarrow> ('a::var,'a,'a raw_term + 'a U,'a raw_term + 'a U) term_pre) \<Rightarrow> 'a U => 'a raw_term" where
+definition suitable ::  "('u \<Rightarrow> ('a, 'a, 'a raw_term + 'u,'a raw_term + 'u) term_pre) \<Rightarrow> bool" where
+  "suitable pick \<equiv> \<forall> d. valid_U d \<longrightarrow> pick d \<in> Utor d"
+definition f :: "('u \<Rightarrow> ('a::var,'a,'a raw_term + 'u,'a raw_term + 'u) term_pre) \<Rightarrow> 'u => 'a raw_term" where
   "f pick \<equiv> corec_raw_term pick"
-
-thm raw_term.corec[of "pick o Utor", unfolded f_def[symmetric]]
+definition pick0 :: "'u \<Rightarrow> ('a, 'a, 'a raw_term + 'u, 'a raw_term + 'u) term_pre" where
+  "pick0 \<equiv> SOME pick. suitable pick"
+definition f0 :: "'u \<Rightarrow> 'a raw_term" where
+  "f0 \<equiv> f pick0"
+definition COREC :: "'u \<Rightarrow> 'a term" where
+  "COREC d = TT_abs (f0 d)"
 
 lemma f_simps:
   "f pick d = raw_term_ctor (map_term_pre id id (case_sum id (f pick)) (case_sum id (f pick)) (pick d))"
@@ -495,38 +362,15 @@ lemma f_ctor:
   by (rule trans[OF assms f_simps, unfolded raw_term.inject])
 
 lemma suitable_FVarsD:
-  assumes "suitable pick"
+  assumes "suitable pick" "valid_U d"
   shows "set1_term_pre (pick d) \<union> \<Union>(case_sum FVars_raw_term raw_UFVars ` set4_term_pre (pick d)) \<union> raw_UFVarsBD (pick d)
        \<subseteq> raw_UFVars d"
-  by (rule allE[OF assms[unfolded suitable_def]])
-    (erule raw_UFVars_Utor)
-
-(*  *)
-
-(* maybe unnecessary *)
-(*lemma f_FVarsD_td:
-  assumes "raw_term_ctor x = f pick d"
-  shows "t \<in> set3_term_pre x \<Longrightarrow> (\<exists>td. t = case_sum id (f pick) td \<and> td \<in> set3_term_pre (pick d))"
-        "t \<in> set4_term_pre x \<Longrightarrow> (\<exists>td. t = case_sum id (f pick) td \<and> td \<in> set4_term_pre (pick d))"
-   apply (unfold f_ctor[OF assms])
-(* REPEAT *)
-  apply (subst (asm) term_pre.set_map, (rule bij_id supp_id_bound)+)
-  apply (erule imageE)
-  apply (rule exI)
-  apply (rule conjI)
-    apply assumption+
-(* REPEAT *)
-  apply (subst (asm) term_pre.set_map, (rule bij_id supp_id_bound)+)
-  apply (erule imageE)
-  apply (rule exI)
-  apply (rule conjI)
-   apply assumption+
-  done
-*)
+  by (rule raw_UFVars_Utor[OF assms(2) assms(1)[unfolded suitable_def, THEN spec, THEN mp, OF assms(2)]])
 
 lemma f_FVarsD_aux:
   assumes "free_raw_term a t"
-    "(\<And>d. t = f pick d \<Longrightarrow> a \<in> raw_UFVars d)"
+    "(\<And>d. valid_U d \<Longrightarrow> t = f pick d \<Longrightarrow> a \<in> raw_UFVars d)"
+    "pred_sum (\<lambda>_. True) valid_U td"
   shows "t = case_sum id (f pick) td \<Longrightarrow> a \<in> case_sum FVars_raw_term raw_UFVars td"
   apply (rule sumE[of td])
    apply hypsubst
@@ -540,46 +384,97 @@ lemma f_FVarsD_aux:
   apply hypsubst
   apply (subst sum.case)
   apply (rule assms(2))
-  apply (hypsubst_thin)
-  apply (subst sum.case)
-  apply (rule refl)
+   apply (unfold sum.simps)
+   apply (insert assms(3))[1]
+   apply hypsubst_thin
+   apply (subst (asm) pred_sum_inject)
+  apply assumption
+  apply assumption
   done
+
+(* TODO: apply-scriptify *)
+lemma valid_pick_set3: "suitable pick \<Longrightarrow> xc \<in> set3_term_pre (pick xb) \<Longrightarrow> valid_U xb \<Longrightarrow> pred_sum (\<lambda>_. True) valid_U xc"
+  apply (unfold suitable_def Utor_def)
+  apply (erule allE)
+  apply (erule impE)
+  apply assumption
+  apply (erule imageE[of _ _ "Udtor xb"])
+  apply (simp only:)
+  apply (subst (asm) term_pre.set_map, (rule supp_id_bound bij_id)+)
+  apply (cases xc)
+  apply hypsubst_thin
+   apply (subst pred_sum.simps)
+   apply simp
+  apply hypsubst_thin
+  apply (subst pred_sum.simps)
+  by (smt (verit, del_insts) UnCI id_apply image_iff insertCI sum.set_map(2) sum_set_simps(4) valid_Udtor')
+
+(* TODO: apply-scriptify *)
+lemma valid_pick_set4: "suitable pick \<Longrightarrow> xc \<in> set4_term_pre (pick xb) \<Longrightarrow> valid_U xb \<Longrightarrow> pred_sum (\<lambda>_. True) valid_U xc"
+  apply (unfold suitable_def Utor_def)
+  apply (erule allE)
+  apply (erule impE)
+  apply assumption
+  apply (erule imageE[of _ _ "Udtor xb"])
+  apply (simp only:)
+  apply (subst (asm) term_pre.set_map, (rule supp_id_bound bij_id)+)
+  apply (cases xc)
+  apply hypsubst_thin
+   apply (subst pred_sum.simps)
+   apply simp
+  apply hypsubst_thin
+  apply (subst pred_sum.simps)
+  by (smt (verit, del_insts) UnCI id_apply image_iff insertCI sum.set_map(2) sum_set_simps(4) valid_Udtor')
 
 lemma f_FVarsD:
   assumes p: "suitable pick"
+and valid_d: "valid_U d"
   shows "FVars_raw_term (f pick d) \<subseteq> raw_UFVars d"
   apply (rule subsetI)
   apply (unfold FVars_raw_term_def mem_Collect_eq)
-  apply (erule free_raw_term.induct[of _ _ "\<lambda>x y. \<forall>d. y = f pick d \<longrightarrow> x \<in> raw_UFVars d", THEN spec, THEN mp[OF _ refl]])
+  apply (erule free_raw_term.induct[of _ _ "\<lambda>x y. \<forall>d. valid_U d \<longrightarrow> y = f pick d \<longrightarrow> x \<in> raw_UFVars d", THEN spec, THEN mp, THEN mp[OF _ refl]])
+     prefer 4
+     apply (rule valid_d)
 
-    apply (rule allI)
-    apply (rule impI)
-    apply (rule le_supE[OF suitable_FVarsD[OF assms, unfolded Un_assoc]])
-    apply (erule subsetD)
+
+     apply (rule allI)
+    apply (rule impI)+
+    apply (rule le_supE[OF suitable_FVarsD[OF assms(1), unfolded Un_assoc]])
+  prefer 2
+     apply (erule subsetD)
     apply (drule f_ctor)
     apply hypsubst
     apply (subst (asm) term_pre.set_map)
       apply (rule supp_id_bound bij_id)+
     apply (unfold image_id)
-    apply assumption
+     apply assumption
+
+  prefer 2
 
 (* REPEAT_DETERM *)
    apply (rule allI)
-   apply (rule impI)
+   apply (rule impI)+
    apply (frule f_ctor)
    apply hypsubst
    apply (subst (asm) term_pre.set_map, (rule supp_id_bound bij_id)+)+
    apply (unfold image_id)?
    apply (erule imageE)
    apply hypsubst
+  thm f_FVarsD_aux
    apply (drule f_FVarsD_aux)
      apply (erule allE)
-     apply (erule impE)
+      apply (erule impE)
+       prefer 2
+  apply (erule impE)
       apply assumption
-     apply assumption
-    apply (rule refl)
+        apply assumption
+  apply assumption
+     prefer 2
+  apply (rule refl)
+     prefer 2
    apply (rule suitable_FVarsD[THEN subsetD, unfolded raw_UFVarsBD_def, rotated]) (* TODO: put union members in correct order *)
-    apply (unfold Un_assoc)
+  apply assumption
+       apply (unfold Un_assoc)
     apply (rule UnI2)
     apply (unfold Un_assoc[symmetric])?
     apply (tactic \<open>resolve_tac @{context} [BNF_Util.mk_UnIN 2 2] 1\<close>) (* normally: Use goal number here *)
@@ -587,34 +482,52 @@ lemma f_FVarsD:
     apply (rule UN_I)
      apply assumption
     apply assumption
-   apply (rule assms)
+     apply (rule assms)
+  prefer 2
+    apply assumption
+   apply (drule valid_pick_set3[OF p])
+    apply assumption
+  apply assumption
     (* repeated *)
-  apply (rule allI)
-  apply (rule impI)
-  apply (frule f_ctor)
-  apply hypsubst
-  apply (subst (asm) term_pre.set_map, (rule supp_id_bound bij_id)+)+
-  apply (unfold image_id)?
-  apply (erule imageE)
-  apply hypsubst
-  apply (drule f_FVarsD_aux)
-    apply (erule allE)
-    apply (erule impE)
+(* TODO: this not actually a repeat anymore, reorganize the proof
+to recover that property *)
+   apply (rule allI)
+   apply (rule impI)+
+   apply (frule f_ctor)
+   apply hypsubst
+   apply (subst (asm) term_pre.set_map, (rule supp_id_bound bij_id)+)+
+   apply (unfold image_id)?
+   apply (erule imageE)
+   apply hypsubst
+  thm f_FVarsD_aux
+   apply (drule f_FVarsD_aux)
+     apply (erule allE)
+      apply (erule impE)
+       prefer 2
+  apply (erule impE)
+      apply assumption
+        apply assumption
+  apply assumption
+     prefer 2
+  apply (rule refl)
+     prefer 2
+   apply (rule suitable_FVarsD[THEN subsetD, unfolded raw_UFVarsBD_def, rotated]) (* TODO: put union members in correct order *)
+  apply assumption
+       apply (unfold Un_assoc)
+    apply (rule UnI2)
+    apply (unfold Un_assoc[symmetric])?
+    apply (tactic \<open>resolve_tac @{context} [BNF_Util.mk_UnIN 2 1] 1\<close>) (* normally: Use goal number here *)
+    apply (rule DiffI[rotated], assumption)?
+    apply (rule UN_I)
      apply assumption
     apply assumption
-   apply (rule refl)
-  apply (rule suitable_FVarsD[THEN subsetD, unfolded raw_UFVarsBD_def, rotated]) (* TODO: put union members in correct order *)
-   apply (unfold Un_assoc)
-   apply (rule UnI2)
-   apply (unfold Un_assoc[symmetric])?
-   apply (tactic \<open>resolve_tac @{context} [BNF_Util.mk_UnIN 2 1] 1\<close>) (* normally: Use goal number here *)
-   apply (rule DiffI[rotated], assumption)?
-   apply (rule UN_I)
-    apply assumption
+   apply (rule assms)
+  apply (rule valid_pick_set4[OF p])
+  prefer 2
    apply assumption
-  apply (rule assms)
-    (* END REPEAT_DETERM *)
+  apply assumption
   done
+    (* END REPEAT_DETERM *)
 
 lemma OO_permute:
   assumes "bij (u::'a\<Rightarrow>'a)" "|supp u| <o |UNIV::'a::var set|"
@@ -642,34 +555,40 @@ lemma OO_permute:
    apply (rule refl)+
   done
 
+
 lemma OO_comp:
-  assumes "g u \<circ> g v = g (u \<circ> v)"
-  shows "(\<lambda>d. (=) (g v d)) OO (\<lambda>d. (=) (g u d)) = (\<lambda>d. (=) (g (u \<circ> v) d))"
+  assumes "\<And>d. valid_U d \<Longrightarrow> (g u \<circ> g v) d = g (u \<circ> v) d"
+  shows "valid_U x \<Longrightarrow> ((\<lambda>d. (=) (g v d)) OO (\<lambda>d. (=) (g u d))) x = (\<lambda>d. (=) (g (u \<circ> v) d)) x"
   apply (subst (2) Grp_UNIV_def[symmetric])
   apply (subst (2) Grp_UNIV_def[symmetric])
   apply (subst Grp_o[symmetric])
   apply (unfold Grp_UNIV_def)
   apply (subst assms)
+  apply assumption
   apply (rule refl)
   done
 
 lemma OO_raw_Umap:
   assumes "bij (u::'a\<Rightarrow>'a)" "|supp u| <o |UNIV::'a::var set|"
           "bij (v::'a\<Rightarrow>'a)" "|supp v| <o |UNIV::'a::var set|"
-        shows "(\<lambda>d. (=) (raw_Umap v d)) OO (\<lambda>d. (=) (raw_Umap u d)) = (\<lambda>d. (=) (raw_Umap (u \<circ> v) d))"
-  by (rule OO_comp[OF Umap_comp0[OF assms]])
+        shows "valid_U x \<Longrightarrow> ((\<lambda>d. (=) (raw_Umap v d)) OO (\<lambda>d. (=) (raw_Umap u d))) x  = (\<lambda>d. (=) (raw_Umap (u \<circ> v) d)) x"
+  apply (rule OO_comp)
+  apply (subst comp_apply)
+   apply (rule Umap_comp[OF _ assms])
+   apply assumption+
+  done
 
 lemma rel_F_suitable_mapD_aux:
-  assumes "suitable pick"
-  shows "X \<in> Utor (d::'a U) \<Longrightarrow> \<exists>v. bij v \<and> |supp v| <o |UNIV::'a::var set| \<and> id_on (raw_UFVarsBD (pick d)) v \<and>
+  assumes "valid_U d" "suitable pick"
+  shows "X \<in> Utor d \<Longrightarrow> \<exists>v. bij v \<and> |supp v| <o |UNIV::'a::var set| \<and> id_on (raw_UFVarsBD (pick d)) v \<and>
       (mr_rel_term_pre id v
         (rel_sum (\<lambda>t. alpha_term (permute_raw_term v t)) (\<lambda>d. (=) (raw_Umap v d)))
         (rel_sum alpha_term (=)) 
         (pick d) X)"
-    apply (rule DTOR_mapD[of "pick d" X d])
+    apply (rule DTOR_mapD[OF assms(1)])
     apply (unfold insert_subset)
     apply (rule conjI)
-     apply (rule assms[unfolded suitable_def, THEN spec])
+     apply (rule assms(2)[unfolded suitable_def, THEN spec, THEN mp, OF assms(1)])
     apply (rule conjI)
     apply assumption
     apply (rule empty_subsetI)
@@ -692,8 +611,10 @@ lemma OO_alpha_permute:
   apply assumption
   done
 
+term mr_rel_term_pre
 lemma rel_F_suitable_mapD:
-  assumes pp': "suitable pick" "suitable pick'"
+  assumes valid_d: "valid_U d"
+    and pp': "suitable pick" "suitable pick'"
     and u: "bij (u::'a\<Rightarrow>'a)" "|supp u| <o |UNIV::'a::var set|"
   shows "\<exists> v. bij v \<and> |supp v| <o |UNIV::'a set| \<and> id_on (raw_UFVarsBD (pick d)) v \<and>
  mr_rel_term_pre u (u o v)
@@ -703,11 +624,13 @@ lemma rel_F_suitable_mapD:
             (\<lambda>d d'. d' = raw_Umap u d))
  (pick d)
  (pick' (raw_Umap u d))"
-  apply (rule raw_Umap_Utor[OF u, of d, unfolded rel_set_def, THEN conjunct2, THEN bspec, THEN bexE])
+  sorry
+(*
+  apply (rule raw_Umap_Utor[OF u valid_d, unfolded rel_set_def, THEN conjunct2, THEN bspec, THEN bexE])
    apply (rule allE)
     apply (rule pp'(2)[unfolded suitable_def])
    apply assumption
-  apply (drule rel_F_suitable_mapD_aux[OF pp'(1)])
+  apply (drule rel_F_suitable_mapD_aux[OF valid_d pp'(1)])
   apply (erule exE)
   apply (erule conjE)+
   apply(rule exI)
@@ -728,8 +651,31 @@ lemma rel_F_suitable_mapD:
             apply (unfold sum.rel_compp[symmetric])
             apply (subst OO_permute[OF u, symmetric])
               apply assumption+
+(*
+            apply (subst rel_sum.simps)
+            apply (subst (asm) rel_sum.simps)
+            apply (erule disjE)
+             apply blast
+            apply (rule disjI2)
+*)
+            (* apply (drule exE)
+  apply (assumption)
+  term rel_sum *)
+            apply (erule sum.rel_cong[OF refl refl, THEN iffD1, rotated -1])
+             apply (rule refl)
+            apply (subst OO_raw_Umap[OF u])
+               apply assumption+
+  thm valid_Udtor'[OF valid_d]
+             apply (rule valid_Udtor'[OF valid_d])
+  apply assumption
+  apply (erule valid_Udtor'[OF valid_d, rotated -1])
+  thm valid_Udtor'[OF valid_d, rotated -1]
+  using valid_Udtor'[OF valid_d]
+  using OO_raw_Umap
+  thm arg_cong2 iffD2 sum.rel_cong[OF refl refl, THEN iffD1]
+  thm OO_raw_Umap[OF u, symmetric]
             apply (subst OO_raw_Umap[OF u, symmetric])
-              apply assumption+
+               apply assumption+
            apply (subst eq_OO)
            apply (rule ballI)+
            apply (rule impI)
@@ -748,6 +694,7 @@ lemma rel_F_suitable_mapD:
      apply (rule supp_comp_bound[OF _ u(2)])
      apply assumption+
   done
+*)
 
 abbreviation (input) "FVarsB x \<equiv> \<Union>(FVars_raw_term ` set3_term_pre x) - set2_term_pre x"
 
@@ -791,9 +738,11 @@ lemma alpha_cong:
 
 lemma f_swap_alpha:
   assumes p: "suitable pick" and p': "suitable pick'"
+   and valid_d: "valid_U d"
   assumes u: "bij (u::'a\<Rightarrow>'a)" "|supp u| <o |UNIV::'a::var set|"
   shows "alpha_term (permute_raw_term u (f pick d)) (f pick' (raw_Umap u d))"
-  apply (rule alpha_coinduct2[of "\<lambda> tL tR. \<exists> u d. bij u \<and> |supp u| <o |UNIV::'a set| \<and>
+  sorry
+(*  apply (rule alpha_coinduct2[of "\<lambda> tL tR. \<exists> u d. valid_U d \<and> bij u \<and> |supp u| <o |UNIV::'a set| \<and>
    tL = permute_raw_term u (f pick d) \<and> tR = f pick' (raw_Umap u d)"])
    apply (rule exI)+
    apply (rule conjI[rotated])+
@@ -805,7 +754,7 @@ lemma f_swap_alpha:
 
 
 proof-
-  let ?\<phi> = "\<lambda> tL tR. \<exists> u d. bij u \<and> |supp u| <o |UNIV::'a set| \<and>
+  let ?\<phi> = "\<lambda> tL tR. \<exists> u d. valid_U d \<and> bij u \<and> |supp u| <o |UNIV::'a set| \<and>
    tL = permute_raw_term u (f pick d) \<and> tR = f pick' (raw_Umap u d)"
   {fix tL tR assume "?\<phi> tL tR"
     hence "alpha_term tL tR"
@@ -815,6 +764,7 @@ proof-
       term un_raw_term_ctor
       then obtain u d
         where u: "bij u" "|supp u| <o |UNIV::'a set|"
+          and valid_d': "valid_U d"
           and "raw_term_ctor xL = permute_raw_term u (f pick d)" "raw_term_ctor xR = f pick' (raw_Umap u d)" by auto
       hence xL: "xL = map_term_pre u u (permute_raw_term u \<circ> case_sum id (f pick)) (permute_raw_term u \<circ> case_sum id (f pick)) (pick d)"
         and xR: "xR = map_term_pre id id (case_sum id (f pick')) (case_sum id (f pick')) (pick' (raw_Umap u d))"
@@ -827,13 +777,16 @@ proof-
        (rel_sum (\<lambda>t. alpha_term (permute_raw_term (u \<circ> v) t)) (\<lambda>d. (=) (raw_Umap (u \<circ> v) d)))
        (rel_sum (\<lambda>t. alpha_term (permute_raw_term u t)) (\<lambda>d d'. d' = raw_Umap u d))
      (pick d) (pick' (raw_Umap u d)) "
-        using rel_F_suitable_mapD[OF p p' u(1,2)] by blast
+        using rel_F_suitable_mapD[OF valid_d' p p' u(1,2)] by blast
       define w where "w \<equiv> u o v o inv u"
       have w: "bij w" "|supp w| <o |UNIV::'a set|" by (simp_all add: w_def u v supp_comp_bound supp_inv_bound)
 
       have fv_xL: "FVarsB xL \<subseteq> u ` (raw_UFVarsBD (pick d))"
         using f_FVarsD[OF p] unfolding xL apply (auto simp: u term_pre.set_map FVars_raw_permutes raw_UFVarsBD_def)
-        subgoal for td a apply (cases td) by fastforce+ .
+        subgoal premises prems for td a 
+          apply (cases td)
+          using prems apply fastforce
+          using prems prems(1)[OF valid_d'] valid_Udtor' oops
       have fv_p'd: "raw_UFVarsBD (pick d) \<subseteq> raw_UFVars d"
         using raw_UFVars_Utor[of "pick d"] p unfolding suitable_def by auto
       have "id_on (u ` (raw_UFVarsBD (pick d))) w"
@@ -896,24 +849,21 @@ proof-
   }
   thus ?thesis using assms by blast
 qed
+*)
 
 lemma f_alpha:
-  assumes p: "suitable pick" and p': "suitable pick'"
+  assumes p: "suitable pick" and p': "suitable pick'" and valid_d: "valid_U d"
   shows "alpha_term (f pick d) (f pick' d)"
-  by (rule f_swap_alpha[OF assms bij_id supp_id_bound, unfolded permute_raw_ids raw_Umap_id])
-
-(*******************************)
-(* Committing to a particular pick function: *)
-
-definition pick0 :: "'a::var U \<Rightarrow> ('a, 'a, 'a raw_term + 'a U, 'a raw_term + 'a U) term_pre" where
-  "pick0 \<equiv> SOME pick. suitable pick"
+  by (rule f_swap_alpha[OF assms bij_id supp_id_bound, unfolded permute_raw_ids raw_Umap_id[OF valid_d]])
 
 lemma exists_suitable:
   "\<exists> pick. suitable pick"
   apply (unfold suitable_def)
   apply (rule choice)
   apply (rule allI)
-  apply (rule ex_in_conv[THEN iffD2, OF Utor_ne])
+  apply (subst ex_simps)
+  apply (rule impI)
+  apply (erule ex_in_conv[THEN iffD2, OF Utor_ne])
   done
 
 lemma suitable_pick0:
@@ -921,13 +871,10 @@ lemma suitable_pick0:
   apply (unfold pick0_def)
   apply (rule someI_ex[OF exists_suitable])
   done
-
-definition "f0 \<equiv> f pick0"
-
 lemmas f0_low_level_simps = f_simps[of pick0, unfolded f0_def[symmetric]]
 
 lemma f0_Utor_aux:
-  assumes "X \<in> Utor d"
+  assumes "X \<in> Utor d" and valid_d: "valid_U d"
   shows "alpha_term (f (\<lambda> d'. if d' = d then X else pick0 d') d)
                        (raw_term_ctor (map_term_pre id id (case_sum id f0) (case_sum id f0) X))"
     apply(subst f_simps)
@@ -950,20 +897,31 @@ lemma f0_Utor_aux:
 
 (* BLOCK: SUITABLE *)
      apply (unfold suitable_def)
-     apply (rule allI)
+    apply (rule allI)
+  apply (rule impI)
      apply (rule if_split[THEN iffD2])
      apply (rule conjI)
       apply (rule impI)
       apply hypsubst
      apply (rule assms)
     apply (rule impI)
-    apply (insert suitable_pick0[unfolded suitable_def])
-    apply (erule allE)
-     apply assumption
+    apply (insert suitable_pick0[unfolded suitable_def, THEN spec, THEN mp])
+    apply assumption
+   apply (rule assms(1)[unfolded Utor_def, THEN imageE])
+   apply (rotate_tac -1)
+   apply (erule valid_Udtor'[rotated])
+     prefer 2
+     apply (rule Basic_BNFs.setr.intros)
+     apply (rule refl)
+     apply hypsubst_thin
+    apply (subst (asm) term_pre.set_map, (rule bij_id supp_id_bound)+)
+(* TODO *)
+    apply (smt (verit, best) Prelim.image_id UnI1 image_iff insertI1 setr.cases sum.set_map(2) sum_set_simps(4))
+  apply (rule assms)
+  
 (* END BLOCK *)
 
-(* REPEATED *)
-     apply (rule sumE)
+(* REPEATED *)     apply (rule sumE)
       apply (frule arg_cong2[OF _ refl, of _ _ "(\<in>)", THEN iffD1])
        apply assumption
       apply hypsubst
@@ -973,51 +931,61 @@ lemma f0_Utor_aux:
       apply hypsubst
      apply (unfold sum.simps)
      apply (unfold f0_def)?
-    apply (rule f_alpha[OF _ suitable_pick0])
+     apply (rule f_alpha[OF _ suitable_pick0])
 
-(* BLOCK: SUITABLE *)
      apply (unfold suitable_def)
-     apply (rule allI)
+    apply (rule allI)
+  apply (rule impI)
      apply (rule if_split[THEN iffD2])
      apply (rule conjI)
       apply (rule impI)
       apply hypsubst
      apply (rule assms)
     apply (rule impI)
-    apply (insert suitable_pick0[unfolded suitable_def])
-    apply (erule allE)
-     apply assumption
-(* END BLOCK *)
+  thm suitable_pick0[unfolded suitable_def, THEN spec, THEN mp]
+    apply (insert suitable_pick0[unfolded suitable_def, THEN spec, THEN mp])
+    apply assumption
+   apply (rule assms(1)[unfolded Utor_def, THEN imageE])
+   apply (rotate_tac -1)
+   apply (erule valid_Udtor'[rotated])
+     prefer 2
+     apply (rule Basic_BNFs.setr.intros)
+     apply (rule refl)
+     apply hypsubst_thin
+    apply (subst (asm) term_pre.set_map, (rule bij_id supp_id_bound)+)
+(* TODO *)
+    apply (smt (verit, best) Prelim.image_id UnI2 image_iff insertI1 setr.cases sum.set_map(2) sum_set_simps(4))
+  apply (rule assms)
 
 (* END REPEAT *)
     done
 
 lemma f0_Utor:
-  assumes "X \<in> Utor d"
+  assumes "X \<in> Utor d" "valid_U d"
   shows "alpha_term (f0 d) (raw_term_ctor (map_term_pre id id (case_sum id f0) (case_sum id f0) X))"
     apply (rule alpha_trans[rotated])
     apply (rule f0_Utor_aux[OF assms])
-    apply (rule f_alpha[OF suitable_pick0, unfolded f0_def[symmetric]])
+    apply (rule f_alpha[OF suitable_pick0 _ assms(2), unfolded f0_def[symmetric]])
 
 (* BLOCK: SUITABLE *)
      apply (unfold suitable_def)
-     apply (rule allI)
+  apply (rule allI)
+  apply (rule impI)
      apply (rule if_split[THEN iffD2])
      apply (rule conjI)
       apply (rule impI)
       apply hypsubst
      apply (rule assms)
     apply (rule impI)
-    apply (insert suitable_pick0[unfolded suitable_def])
-    apply (erule allE)
+    apply (insert suitable_pick0[unfolded suitable_def, THEN spec, THEN mp])
      apply assumption
 (* END BLOCK *)
   done
 
 lemma f0_mapD:
-  assumes "bij (u::'a\<Rightarrow>'a)" and "|supp u| <o |UNIV::'a::var set|"
+  assumes "bij (u::'a\<Rightarrow>'a)" and "|supp u| <o |UNIV::'a::var set|" "valid_U d"
   shows "alpha_term (f0 (raw_Umap u d)) (permute_raw_term u (f0 d))"
-  by (rule alpha_syms[OF f_swap_alpha[OF suitable_pick0 suitable_pick0 assms, unfolded f0_def[symmetric]]])
+  by (rule alpha_syms[OF f_swap_alpha[OF suitable_pick0 suitable_pick0 assms(3,1,2), unfolded f0_def[symmetric]]])
 
 lemmas f0_FVarsD = f_FVarsD[OF suitable_pick0, unfolded f0_def[symmetric]]
 
@@ -1026,13 +994,12 @@ lemmas f0_FVarsD = f_FVarsD[OF suitable_pick0, unfolded f0_def[symmetric]]
 thm f0_Utor f0_mapD f0_FVarsD
 
 
-
 (*******************)
 (* End product: *)
-definition ff0 :: "'a::var U \<Rightarrow> 'a term" where "ff0 d = TT_abs (f0 d)"
+definition ff0 :: "'u \<Rightarrow> 'a term" where "ff0 d = TT_abs (f0 d)"
 
 theorem ff0_DDTOR:
-  assumes "X \<in> Udtor d"
+  assumes "X \<in> Udtor d" "valid_U d"
   shows "ff0 d = term_ctor (map_term_pre id id (case_sum id ff0) (case_sum id ff0) X)"
   apply (unfold ff0_def term_ctor_def)
   apply (unfold o_def[symmetric])
@@ -1046,7 +1013,7 @@ theorem ff0_DDTOR:
     apply (rule f0_Utor)
     apply (unfold Utor_def)
     apply (rule imageI)
-    apply (rule assms)
+     apply (rule assms)+
    apply (subst term_pre.map_comp, (rule supp_id_bound bij_id)+)
    apply (unfold case_sum_o_map_sum)
    apply (unfold id_comp comp_id)
@@ -1083,25 +1050,31 @@ theorem ff0_DDTOR:
   apply (rule TT_rep_abs_syms)
   done
 
-
 lemma ff0_mmapD:
-  assumes "bij (u::'a\<Rightarrow>'a)" and "|supp u| <o |UNIV::'a::var set|"
+  assumes "bij (u::'a\<Rightarrow>'a)" and "|supp u| <o |UNIV::'a::var set|" and "valid_U d"
   shows "ff0 (Umap u d) = permute_term u (ff0 d)"
   apply (unfold ff0_def permute_term_def)
   apply (unfold TT_total_abs_eq_iffs)
   apply (rule alpha_trans)
-   apply (rule f0_mapD[OF assms, of d])
-  apply (unfold alpha_bij_eqs[OF assms])
+   apply (rule f0_mapD[OF assms])
+  apply (unfold alpha_bij_eqs[OF assms(1,2)])
   apply (rule alpha_syms)
   apply (rule TT_rep_abs)
   done
 
 theorem ff0_FFVarsD:
-  "FVars_term (ff0 d) \<subseteq> UFVars d"
+  "valid_U d \<Longrightarrow> FVars_term (ff0 d) \<subseteq> UFVars d"
   apply (unfold ff0_def FVars_term_def alpha_FVars[OF TT_rep_abs])
-  apply (rule f0_FVarsD)
+  apply (erule f0_FVarsD)
   done
 
-hide_const f
+lemma COREC_DDTOR: "valid_U d \<Longrightarrow> X \<in> Udtor d \<Longrightarrow> COREC d = term_ctor (map_term_pre id id (case_sum id COREC) (case_sum id COREC) X)"
+  sorry
+
+  lemma COREC_mmapD: "valid_U d \<Longrightarrow> bij u \<Longrightarrow> |supp u| <o |UNIV::'a set| \<Longrightarrow> COREC (Umap u d) = permute_term u (COREC d)"
+    sorry
+  lemma  COREC_FFVarsD: "valid_U d \<Longrightarrow> FVars_term (COREC d) \<subseteq> UFVars d"
+    sorry
+end
 
 end
